module ch3-my-nat-thms where

open import ial.bool
open import ial.bool-thms
open import ial.bool-thms2
open import ial.eq
open import ial.nat
open import ial.nat-thms
open import ial.neq
open import ial.product
open import ial.product-thms
open import ial.sum


-- 1. Pick some theorems in nat-thms and reprove them yourself.
-- + is commutative
+commâ€² : âˆ€ (x y : â„•) â†’ x + y â‰¡ y + x
+commâ€² zero y rewrite +0 y = refl
+commâ€² (suc x) y rewrite +suc y x | +commâ€² x y = refl

+permâ€² : âˆ€ (x y z : â„•) â†’ x + (y + z) â‰¡ y + (x + z)
+permâ€² zero y z rewrite +commâ€² y z  = refl
+permâ€² (suc x) y z rewrite +permâ€² x y z | +suc y (x + z) = refl


{-
  2. In nat.agda, greather-than and greather-than-or-equal-to orderings are defined in terms of less-than and less-than-or-equal-to.
     Prove versions of theorems like <-trans and <+, but modified to use _>_ instead of _<_ .
-}

aux : âˆ€ (n : â„•) â†’ 0 < (suc n) â‰¡ tt
aux zero = refl
aux (suc x) = refl

<-transâ€² : âˆ€ {x y z : â„•} â†’ x > y â‰¡ tt â†’ y > z â‰¡ tt â†’ x > z â‰¡ tt
<-transâ€² {x} {0} {z} ()
<-transâ€² {0} {suc y} {0} ()
<-transâ€² {0} {suc y} {suc z} ()
<-transâ€² {suc x} {suc y} {0} p1 p2 = aux x
<-transâ€² {suc x} {suc y} {suc z} p1 p2 = {!TODO!}
{-
   3. For each of the following functions, which one statement describes best what
      the function f does? There is exactyle one correct answer for each.
-}

-- (a)
f : (n : â„•) â†’ â„•
f 0 = 1
f (suc x) = (suc x) * (f x)

{-
  1. Reverses a list
  2. Multiplies input n by itself
  3. Computes n^n
  4. Computes factorial
-}

-- Answer: 4. f n computes n's factorial

-- (b)
fâ€² : â„• â†’ ð”¹
fâ€²â€² : (n : â„•) â†’ ð”¹
fâ€²â€² 0 = tt
fâ€²â€² (suc x) = fâ€² x
fâ€² 0 = ff
fâ€² (suc x) = fâ€²â€² x

{-
  1. Returns tt (boolean true) iff n is even
  2. Returns tt iff n is 0
  3. Return tt iff n is odd
  4. Returns the length of n
  5. Computes primality of n
-}

-- Answer: 1. fâ€²â€² returns tt iff n is even. Let fâ€² = f1 and fâ€²â€² = f2:
f1 : â„• â†’ ð”¹
f2 : (n : â„•) â†’ ð”¹
f2 0 = is-even 0
f2 (suc x) = is-odd x
f1 0 = ff
f1 (suc x) = is-even x

